Fix the semantics of Bind. Prove wp rules for bind, loop, and StatDb spinlock.
It used to be the case that 'Ret v' could take a dummy step, so when stepping a
'Bind e f', we would always first step e, then check if the result was a Ret
and do the substitution if necessary. That's a bit strange and makes it hard to
prove the expected sequencing rule for Bind.

Now, Ret does not take a step, and the rule for Bind cases on whether e is a
Ret or not.

src/Examples/StatDb/WeakestPre.v
@@ -3,20 +3,21 @@ Require Export CSL.WeakestPre.
 Require Import CSL.Lifting.
 Require Import StatDb.Impl.
 Require Import Helpers.RelationTheorems.
+From iris.base_logic.lib Require Export invariants.
 From iris.proofmode Require Import tactics.
 Set Default Proof Using "Type".
 
 
-Class statG Σ := StatG {
-                     stat_invG : invG Σ;
-                     stat_alg_inG :> inG Σ (authR (optionUR (exclR natC)));
-                     stat_reg_gnames: Var.id -> gname
+Class varG Σ := VarG {
+                     var_invG : invG Σ;
+                     var_alg_inG :> inG Σ (authR (optionUR (exclR natC)));
+                     var_reg_gnames: Var.id -> gname
                    }.
 
-Definition reg_map `{statG Σ} (i: Var.id) (v: nat) :=
-  own (stat_reg_gnames i) (◯ (Excl' v)).
-Definition reg_map_auth `{statG Σ} (i: Var.id) (v: nat) :=
-  own (stat_reg_gnames i) (● (Excl' v)).
+Definition reg_map `{varG Σ} (i: Var.id) (v: nat) :=
+  own (var_reg_gnames i) (◯ (Excl' v)).
+Definition reg_map_auth `{varG Σ} (i: Var.id) (v: nat) :=
+  own (var_reg_gnames i) (● (Excl' v)).
 
 Local Notation "i ↦ v" := (reg_map i v) (at level 20) : bi_scope.
 Local Notation "i ↦● v" := (reg_map_auth i v) (at level 20) : bi_scope.
@@ -24,15 +25,15 @@ Local Notation "i ↦● v" := (reg_map_auth i v) (at level 20) : bi_scope.
 
 Import Var.
 
-Instance statG_irisG `{statG Σ} : irisG Var.Op Var.l Σ :=
+Instance varG_irisG `{varG Σ} : irisG Var.Op Var.l Σ :=
   {
-    iris_invG := stat_invG;
+    iris_invG := var_invG;
     state_interp := (λ '(ns, nc, nl), Var.Sum ↦● ns ∗ Var.Count ↦● nc ∗ Var.Lock ↦● nl)%I
   }.
 
 
 Section lifting.
-Context `{statG Σ}.
+Context `{varG Σ}.
 
 Lemma reg_update i vnew v1 v2 : i ↦ v1 -∗ i ↦● v2 ==∗ i ↦ vnew ∗ i ↦● vnew.
 Proof.
@@ -48,6 +49,9 @@ Proof.
     by iDestruct (own_valid_2 with "Ha Hf")
       as %[<-%Excl_included%leibniz_equiv _]%auth_valid_discrete_2.
 Qed.
+
+Global Instance reg_map_timless i v: Timeless (i ↦ v).
+Proof. apply _. Qed.
 
 Ltac destruct_state σ H :=
   destruct σ as ((?&?)&?);
@@ -124,3 +128,66 @@ Proof.
 Qed.
 
 End lifting.
+
+(* Essentially the same as the verification of the spinlock in Iris heap_lang
+   except we don't allocate locks or pass the pointer to them; there is a dedicated
+   lock register. *)
+
+Class lockG Σ := LockG { lock_tokG :> inG Σ (exclR unitC) }.
+Definition lockΣ : gFunctors := #[GFunctor (exclR unitC)].
+Instance subG_lockΣ {Σ} : subG lockΣ Σ → lockG Σ.
+Proof. solve_inG. Qed.
+
+Section lock.
+  Context `{!varG Σ, !lockG Σ}.
+
+  Definition lock_inv (γ : gname) (P : iProp Σ) : iProp Σ :=
+    ((Lock ↦ 0 ∗ P ∗ own γ (Excl ())) ∨ (Lock ↦ 1))%I.
+
+  Definition is_lock (N: namespace) (γ: gname) (P: iProp Σ) : iProp Σ :=
+    (inv N (lock_inv γ P))%I.
+
+  Definition locked (γ: gname) : iProp Σ :=
+    own γ (Excl ()).
+
+  Global Instance is_lock_persistent N γ R : Persistent (is_lock N γ R).
+  Proof. apply _. Qed.
+
+  Global Instance locked_timless γ : Timeless (locked γ).
+  Proof. apply _. Qed.
+
+  Lemma lock_init N (R: iProp Σ) E : Lock ↦ 0 -∗ R ={E}=∗ ∃ γ, is_lock N γ R.
+  Proof.
+    iIntros "Hl HR".
+    iMod (own_alloc (Excl ())) as (γ) "Hexcl"; first done.
+    iMod (inv_alloc N _ (lock_inv γ R) with "[-]").
+    { iNext. iLeft; iFrame. }
+    iModIntro; iExists _; done.
+  Qed.
+
+  Lemma wp_lock N γ (R: iProp Σ):
+    {{{ is_lock N γ R }}} lock {{{ RET tt; locked γ ∗ R }}}.
+  Proof.
+    iIntros (Φ) "#Hlock HΦ". iLöb as "IH".
+    wp_loop; wp_bind.
+    iInv N as "[HL|>HUL]".
+    - iDestruct "HL" as "(>H&?&>?)".
+      iApply (wp_cas_suc with "[$]"). iIntros "!> Hl !>"; iFrame.
+      rewrite //=. wp_ret. wp_ret.
+      iApply "HΦ"; iFrame.
+    - iApply (wp_cas_fail with "[$]"); first done. iIntros "!> Hl !>"; iFrame.
+      rewrite //=. wp_ret. iApply "IH"; eauto.
+  Qed.
+
+  Lemma wp_unlock N γ (R: iProp Σ):
+    {{{ is_lock N γ R ∗ locked γ ∗ R }}} unlock {{{ RET tt; True }}}.
+  Proof.
+    iIntros (Φ) "(#Hlock&Hlocked&HR) HΦ".
+    iInv N as "[HL|>HUL]".
+    - iDestruct "HL" as "(>H&?&>Htok)".
+      iDestruct (own_valid_2 with "Htok Hlocked") as %H => //=.
+    - iApply (wp_write with "[$]"); iIntros "!> H !>".
+      iSplitR "HΦ"; last by iApply "HΦ".
+      iLeft. iFrame.
+  Qed.
+End lock.
